conn/props.v
@@ -71,116 +71,6 @@ Definition wf_sess_info rl si : iProp :=
 Instance wf_sess_info_persistent rl si : Persistent (wf_sess_info rl si).
 Proof. apply _. Qed.
 
-Definition session_failed_for si rl (failed : bool) : iProp :=
-  term_meta (si_share_of rl si) (isoN.@"failed") failed ∗
-  (if failed then failure (si_init si) (si_resp si)
-   else □ (public (si_key si) ↔ ▷ released_session si))%I.
-
-#[global]
-Instance session_failed_for_persistent si rl failed :
-  Persistent (session_failed_for si rl failed).
-Proof. by apply _. Qed.
-
-Lemma session_failed_for_agree si rl failed1 failed2 :
-  session_failed_for si rl failed1 -∗
-  session_failed_for si rl failed2 -∗
-  ⌜failed1 = failed2⌝.
-Proof.
-iIntros "(#meta1 & _) (#meta2 & _)".
-iApply (term_meta_agree with "meta1 meta2").
-Qed.
-
-Definition session_failed si failed : iProp :=
-  if failed then
-    (session_failed_for si Init true ∨
-     session_failed_for si Resp true)%I
-  else
-    (session_failed_for si Init false ∗
-     session_failed_for si Resp false)%I.
-
-Lemma session_failedI si failed1 failed2 :
-  session_failed_for si Init failed1 -∗
-  session_failed_for si Resp failed2 -∗
-  session_failed si (failed1 || failed2).
-Proof.
-iIntros "#? #?".
-case: failed1 => //=; eauto.
-case: failed2 => //=; eauto.
-Qed.
-
-Lemma session_failedI' si rl failed1 failed2 :
-  session_failed_for si rl failed1 -∗
-  session_failed_for si (swap_role rl) failed2 -∗
-  session_failed si (failed1 || failed2).
-Proof.
-iIntros "#failed1 #failed2". case: rl.
-- iApply (session_failedI with "failed1 failed2").
-- rewrite Bool.orb_comm. iApply (session_failedI with "failed2 failed1").
-Qed.
-
-Lemma session_okI si failed :
-  session_failed si failed -∗
-  (failure (si_init si) (si_resp si) -∗ ▷ False) -∗
-  ◇ session_failed si false.
-Proof.
-case: failed => //; eauto.
-by iIntros "#[[_ fail1]|[_ fail2]] contra";
-iDestruct ("contra" with "[]") as ">[]".
-Qed.
-
-#[global]
-Instance session_failed_persistent si failed :
-  Persistent (session_failed si failed).
-Proof. apply _. Qed.
-
-Lemma session_failed_agree si failed1 failed2 :
-  session_failed si failed1 -∗
-  session_failed si failed2 -∗
-  ⌜failed1 = failed2⌝.
-Proof.
-iIntros "#failed1 #failed2".
-iAssert (session_failed si true -∗
-         session_failed si false -∗ False)%I
-  as "P".
-{ iIntros "#[fail|fail] #[succ1 succ2]".
-  - by iPoseProof (session_failed_for_agree with "fail succ1") as "%".
-  - by iPoseProof (session_failed_for_agree with "fail succ2") as "%". }
-case: failed1 failed2 => [] [] //.
-- by iDestruct ("P" with "failed1 failed2") as "[]".
-- by iDestruct ("P" with "failed2 failed1") as "[]".
-Qed.
-
-Lemma session_failed_forI rl cs (P : iProp) (failed : bool) :
-  wf_sess_info rl cs -∗
-  (if failed then failure (si_init cs) (si_resp cs) else P) -∗
-  term_token (cs_share cs) (↑isoN) ==∗ ∃ failed',
-  ⌜failed → failed'⌝ ∗
-  session_failed_for cs (cs_role cs) failed' ∗
-  (⌜failed'⌝ ∨ P) ∗
-  term_token (cs_share cs) (↑isoN ∖ ↑isoN.@"failed").
-Proof.
-iIntros "#wf HP token".
-iPoseProof "wf" as "(_ & _ & #? & %failed' & #failed' & ?)".
-case: failed'.
-{ iMod (term_meta_set' true (N := isoN.@"failed") with "token")
-    as "[#failed token]" => //; try solve_ndisj.
-  iAssert (session_failed_for cs (cs_role cs) true) as "#?".
-  { iSplit => //. }
-  iExists true. iModIntro. iFrame. do !iSplit => //; eauto. }
-case: failed.
-{ iPoseProof "HP" as "#fail".
-  iMod (term_meta_set' true (N := isoN.@"failed") with "token")
-    as "[#failed token]" => //; try solve_ndisj.
-  iFrame "token". iModIntro. iExists true.
-  do !iSplit => //; eauto. }
-iMod (term_meta_set' false (N := isoN.@"failed") with "token")
-  as "[#failed token]" => //; try solve_ndisj.
-iAssert (session_failed_for cs (cs_role cs) false) as "#?".
-{ iSplit => //. iModIntro. by iSplit => //. }
-iFrame "token". iModIntro. iExists false.
-do !iSplit => //; eauto.
-Qed.
-
 Definition never_connected kI kR : iProp :=
   term_token kR (↑N.@"server".@kI).
 
@@ -232,9 +122,9 @@ Definition server_clock_ready kI kR :=
   escrow nroot (never_connected kI kR)
     (clock kI kR 0).
 
-Definition client_disconnected kI kR n failed : iProp :=
+Definition client_disconnected kI kR n : iProp :=
   server_clock_ready kI kR ∗
-  if failed then failure kI kR else clock kI kR n.
+  (failure kI kR ∨ clock kI kR n).
 
 Definition client_disconnecting kI kR cs : iProp :=
   ⌜cs_role cs = Init⌝ ∗
@@ -245,11 +135,9 @@ Definition connected' kI kR cs b n n0 : iProp :=
   ⌜si_init cs = kI⌝ ∗
   ⌜si_resp cs = kR⌝ ∗
   wf_sess_info (cs_role cs) cs ∗
-  (∃ failed, session_failed_for cs (cs_role cs) failed) ∗
   (if b then released (cs_share cs) else release_token (cs_share cs)) ∗
   cs_ts cs ↦ #n ∗
-  (∃ failed, session_failed cs failed) ∗
-  (session_failed cs true ∨
+  (compromised_session (cs_role cs) cs ∨
      term_meta (si_init_share cs) (isoN.@"beginning") n0).
 
 Definition connected kI kR cs n : iProp :=
@@ -267,91 +155,51 @@ Definition client_token kI kR cs : iProp :=
   server_clock_ready kI kR ∗
   term_token (si_init_share cs) (↑isoN.@"end").
 
-Definition client_connecting cs n0 failed : iProp :=
+Definition client_connecting cs n0 : iProp :=
   let kI := si_init cs in
   let kR := si_resp cs in
   server_clock_ready kI kR ∗
   wf_sess_info Init cs ∗
   term_meta  (si_init_share cs) (isoN.@"beginning") n0 ∗
-  term_token (si_init_share cs) (↑isoN.@"end") ∗
-  session_failed_for cs Init failed.
-
-Lemma client_connecting_failed cs n0 failed :
-  client_connecting cs n0 failed -∗
-  session_failed_for cs Init failed.
-Proof. by iIntros "(_ & _ & _ & _ & ?)". Qed.
+  term_token (si_init_share cs) (↑isoN.@"end").
 
 Definition conn_ready si n :=
   escrow nroot
          (term_token (si_resp_share si) (↑isoN.@"begin"))
          (clock (si_init si) (si_resp si) n).
 
-Lemma client_connectingI kI kR cs beginning failed :
-  si_init cs = kI →
-  si_resp cs = kR →
+Lemma client_connectedI cs n0 :
   cs_role cs = Init →
-  cryptis_ctx -∗
-  £ 1 ∗ £ 1 -∗
-  wf_sess_info Init cs -∗
-  term_token (si_init_share cs) (↑isoN) -∗
-  client_disconnected kI kR beginning failed ={⊤}=∗ ∃ failed',
-  ⌜failed → failed'⌝ ∗
-  client_connecting cs beginning failed' ∗
-  term_meta (si_init_share cs) (isoN.@"beginning") beginning ∗
-  (⌜failed'⌝ ∨ conn_ready cs beginning).
-Proof.
-move=> <- <- e_rl {kI kR}.
-iIntros "#? [c1 c2] #sess token dis".
-iDestruct "dis" as "(#server & status)".
-have e_sh : si_init_share cs = cs_share cs by rewrite /cs_share e_rl.
-rewrite e_sh.
-iMod (session_failed_forI with "sess status token")
-  as "(%failed' & % & #conn & status & token)".
-iMod (term_meta_set' (N:=isoN.@"beginning") beginning with "token")
-  as "[#beginning token]"; try solve_ndisj.
-iExists failed'. iSplitR => //. iSplitL "token" => //.
-{ rewrite /client_connecting e_sh e_rl. iModIntro. do !iSplit => //.
-  rewrite (term_token_difference _ (↑isoN.@"end")); try solve_ndisj.
-  iDestruct "token" as "[token' token]". iFrame "token'". }
-iSplitR => //.
-iDestruct "status" as "[#?|status]"; eauto.
-iRight. iApply (escrowI with "status"). iApply term_token_switch.
-Qed.
-
-Lemma client_connectedI cs n0 failedI failedR :
-  cs_role cs = Init →
-  client_connecting cs n0 failedI -∗
+  client_connecting cs n0 -∗
   cs_ts cs ↦ #0%nat -∗
-  release_token (si_init_share cs) -∗
-  session_failed_for cs Resp failedR ={⊤}=∗
+  release_token (si_init_share cs) ={⊤}=∗
   ▷ (connected (si_init cs) (si_resp cs) cs n0 ∗
      client_token (si_init cs) (si_resp cs) cs).
 Proof.
-iIntros "%e_rl (#server & #? & #? & ? & #conn) ts rel #status".
+iIntros "%e_rl (#server & #? & #? & ?) ts rel".
 rewrite /connected /connected' /client_token /cs_share e_rl /=.
 iFrame. do 2!iModIntro. iSplit; last by do 4!iSplit => //.
-iExists n0. do 6!iSplit => //; eauto.
-iSplit; eauto.
-iExists (failedI || failedR).
-case: failedI => /=; eauto.
-case: failedR => /=; eauto.
+iExists n0. do 4!iSplit => //; eauto.
 Qed.
 
 Lemma connected_ok kI kR cs n :
   connected kI kR cs n -∗
-  (failure kI kR -∗ ▷ False) -∗
-  ◇ session_failed cs false.
+  secret kI -∗
+  secret kR -∗
+  sign_key kI -∗
+  sign_key kR -∗
+  ◇ □ ¬ compromised_session (cs_role cs) cs.
 Proof.
-iIntros "(% & % & % & _ & conn) post".
-iDestruct "conn"
-  as "(<- & <- & #conn & #? & rel & ts & #(%failed & status) & _)".
-by iDestruct (session_okI with "status post") as ">?".
+iIntros "(% & % & % & _ & conn) s_kI s_kR #signI #signR".
+iDestruct "conn" as "(<- & <- & #conn & rel & _)".
+iDestruct "conn" as "(m_k & s_k & sess)".
+by iApply (session_not_compromised with "[//] s_kI s_kR").
 Qed.
 
 Lemma client_alloc kI kR E :
   ↑N.@"client".@kR.@"clock" ⊆ E →
   term_token kI E ={⊤}=∗
-  client_disconnected kI kR 0 false ∗
+  client_disconnected kI kR 0 ∗
   term_token kI (E ∖ ↑N.@"client".@kR.@"clock").
 Proof.
 iIntros "%sub kI_token".
@@ -367,146 +215,52 @@ Qed.
 
 Definition server_token cs : iProp :=
   ⌜cs_role cs = Resp⌝ ∗
-  (session_failed cs true ∨ ∃ n0,
+  (compromised_session Resp cs ∨ ∃ n0,
      clock (si_init cs) (si_resp cs) n0 ∗
      clock (si_init cs) (si_resp cs) n0).
 
-Definition server_disconnected kI kR n failed : iProp :=
-  if failed then failure kI kR
-  else (⌜n = 0⌝ ∗ never_connected kI kR ∨ clock kI kR n)%I.
+Definition server_disconnected kI kR n : iProp :=
+  failure kI kR ∨
+  (⌜n = 0⌝ ∗ never_connected kI kR ∨ clock kI kR n).
 
 Lemma server_alloc kI kR E :
   ↑N.@"server".@kI ⊆ E →
   term_token kR E ==∗
-  server_disconnected kI kR 0 false ∗
+  server_disconnected kI kR 0 ∗
   term_token kR (E ∖ ↑N.@"server".@kI).
 Proof.
 iIntros "%sub token".
 rewrite (term_token_difference _ (↑N.@"server".@kI)) //.
 iDestruct "token" as "[token ?]". iFrame.
-iModIntro. iLeft. by eauto.
+iModIntro. iRight. iLeft. by eauto.
 Qed.
 
-Definition session_msg_pred (Q : sess_info → term → iProp) rl kS m : iProp :=
-  ∃ si failed,
-    ⌜kS = (si_key si)⌝ ∗ public m ∗ session_failed_for si rl failed ∗
-    (⌜failed⌝ ∨ Q si m).
+Definition session_msg_pred (Q : sess_info → term → iProp) kS m : iProp :=
+  ∃ si, ⌜kS = (si_key si)⌝ ∗ public m ∗ Q si m.
 
 Definition init_pred si t : iProp := ∃ (beginning : nat),
   server_clock_ready (si_init si) (si_resp si) ∗
   term_meta (si_init_share si) (isoN.@"beginning") beginning ∗
   conn_ready si beginning.
 
-Lemma init_predI cs beginning failed m :
-  client_connecting cs beginning failed -∗
-  ⌜failed⌝ ∨ conn_ready cs beginning -∗
-  □ (⌜failed⌝ ∨ init_pred cs m).
+Lemma init_predI cs beginning m :
+  client_connecting cs beginning -∗
+  compromised_session Init cs ∨ conn_ready cs beginning -∗
+  □ (compromised_session Init cs ∨ init_pred cs m).
 Proof.
-iIntros "(#server & #? & #? & ? & ? & #status) #[fail|ready]"; eauto.
+iIntros "(#server & #? & #? & ?) #[fail|ready]"; eauto.
 iModIntro. iRight. iExists _. eauto 10.
-Qed.
-
-Definition incoming_connection kR cs : iProp :=
-  wf_sess_info Resp cs ∗
-  cs_ts cs ↦ #0%nat ∗
-  ⌜si_resp cs = kR⌝ ∗
-  ⌜cs_role cs = Resp⌝ ∗
-  release_token (cs_share cs) ∗
-  term_token (si_resp_share cs) (↑isoN) ∗
-  (∀ failed,
-     release_token (cs_share cs) -∗
-     session_failed_for cs (cs_role cs) failed ={⊤}=∗ ∃ failed',
-     ⌜failed → failed'⌝ ∗
-     release_token (cs_share cs) ∗
-     session_failed cs failed' ∗
-     (⌜failed'⌝ ∨ ∃ m, init_pred cs m)).
-
-Lemma server_connect kR cs n0 failed :
-  server_disconnected (si_init cs) kR n0 failed -∗
-  incoming_connection kR cs ={⊤}=∗
-  □ (⌜failed⌝ -∗ session_failed cs true) ∗
-  connected (si_init cs) kR cs n0 ∗
-  server_token cs.
-Proof.
-iIntros "dis (#sess & ts & <- & %e_rl & rel & token & close)".
-have ->: si_resp_share cs = cs_share cs.
-{ by rewrite /cs_share e_rl. }
-iMod (session_failed_forI with "sess dis token")
-  as "(%failed' & %le_failed & #failed & dis & token)".
-iMod ("close" with "rel failed")
-  as "(%failed'' & %le_failed' & rel & #failed' & #init)".
-rewrite /connected /connected' /cs_share e_rl /=.
-iMod (term_meta_set' (N := isoN.@"beginning") n0
-       with "token") as "[#beginning token]"; try solve_ndisj.
-rewrite (term_token_difference _ (↑isoN.@"begin")); try solve_ndisj.
-iDestruct "token" as "[token _]".
-iDestruct "dis" as "[%fail|dis]".
-{ iAssert (session_failed cs true) as "#?".
-  { by case: failed'' => //= in le_failed' *. }
-  iFrame. do !iSplitR => //; eauto.
-  iExists n0. do !iSplitR => //; eauto. }
-iDestruct "init" as "[%fail|(%m & init)]".
-{ case: failed'' {le_failed'} => // in fail *.
-  iFrame. do !iSplitR => //; eauto.
-  iExists n0. do !iSplitR => //; eauto. }
-iDestruct "init" as "(%n0' & clock & beginningI & ready)".
-iMod (escrowE with "ready token") as ">c1" => //.
-iAssert (|={⊤}=> clock (si_init cs) (si_resp cs) n0)%I
-  with "[dis]" as "> c2".
-{ iDestruct "dis" as "[(-> & never)|c2]" => //.
-  iMod (escrowE with "clock never") as ">?" => //. }
-iPoseProof (clock_agree with "c1 c2") as "->".
-iModIntro. iFrame. do !iSplit => //; eauto.
-- iIntros "!> %fail".
-  have: failed'' by tauto.
-  by case: (failed'').
-- iExists n0. do !iSplit => //; eauto.
-- iRight. iFrame.
 Qed.
 
 Definition ack_init_pred si t : iProp := True.
 
 Definition conn_pred φ kS m : iProp :=
-  ∃ si n ts,
+  ∃ si n ts n0,
     ⌜kS = si_key si⌝ ∗
     ⌜m = Spec.of_list (TInt n :: ts)⌝ ∗
     ([∗ list] t ∈ ts, public t) ∗
-    (∃ failed, session_failed si failed) ∗
-    (session_failed si true ∨ ∃ n0,
-      term_meta (si_init_share si) (isoN.@"beginning") n0 ∗
-      φ (si_init si) (si_resp si) si (n + n0) ts).
-
-Lemma conn_predI kI kR cs b m n0 φ n ts :
-  connected' kI kR cs b m n0 -∗
-  ([∗ list] t ∈ ts, public t) -∗
-  □ (session_failed cs true ∨ φ kI kR (cs_si cs) (n + n0) ts) -∗
-  □ conn_pred φ (si_key cs) (Spec.of_list (TInt n :: ts)).
-Proof.
-iIntros "(<- & <- & #conn & #? & _ & _ & #failed & #beginning)".
-iIntros "#p_ts #inv !>".
-iExists cs, n, ts.
-do 4!iSplit => //.
-iDestruct "beginning" as "[?|beginning]"; eauto.
-iDestruct "inv" as "[?|inv]"; eauto.
-Qed.
-
-Lemma conn_predE kI kR cs b m n n0 φ ts :
-  connected' kI kR cs b m n0 -∗
-  □ conn_pred φ (si_key cs) (Spec.of_list (TInt n :: ts)) -∗
-  ([∗ list] t ∈ ts, public t) ∗
-  □ (session_failed cs true ∨ φ kI kR (cs_si cs) (n + n0) ts).
-Proof.
-iIntros "(<- & <- & #conn & #? & _ & _ & #failed & #beginning)".
-iIntros "#(%si & %n' & %ts' & %e_kS & %e_m & p_ts & failed' & inv)".
-case/Spec.of_list_inj: e_m => e_n <-.
-have {e_n} ?: n = n' by lia. subst n'.
-rewrite -(session_agree e_kS) {e_kS}.
-iSplit => //. iModIntro.
-iDestruct "beginning" as "[?|beginning]"; eauto.
-iDestruct "inv" as "[?|(%n0' & beginning' & inv)]"; eauto.
-iPoseProof (term_meta_agree with "beginning beginning'") as "<-".
-by iRight.
-Qed.
+    term_meta (si_init_share si) (isoN.@"beginning") n0 ∗
+    φ (si_init si) (si_resp si) si (n + n0) ts.
 
 Definition close_pred kI kR si n ts : iProp :=
   True.
@@ -520,17 +274,13 @@ Definition ack_close_pred kI kR si n ts : iProp :=
   conn_closed si n ∗
   released (si_resp_share si).
 
-Lemma session_failed_failure si failed :
-  session_failed si failed ⊢ ⌜failed⌝ → failure (si_init si) (si_resp si).
-Proof.
-iIntros "#failed %fail".
-case: failed in fail * => //=.
-by iDestruct "failed" as "[[_ fail]|[_ fail]]".
-Qed.
+Lemma session_failed_failure rl si :
+  compromised_session rl si  ⊢ failure (si_init si) (si_resp si).
+Proof. by iIntros "(#failed & _)". Qed.
 
 Definition ctx : iProp :=
-  seal_pred  (N.@"conn".@"init")      (session_msg_pred init_pred Init) ∗
-  seal_pred  (N.@"conn".@"ack_init")  (session_msg_pred ack_init_pred Resp) ∗
+  seal_pred  (N.@"conn".@"init")      (session_msg_pred init_pred) ∗
+  seal_pred  (N.@"conn".@"ack_init")  (session_msg_pred ack_init_pred) ∗
   seal_pred  (N.@"conn".@"close")     (conn_pred close_pred) ∗
   seal_pred  (N.@"conn".@"ack_close") (conn_pred ack_close_pred) ∗
   iso_dh_ctx (N.@"conn".@"auth").
@@ -568,11 +318,11 @@ Ltac solve_ctx :=
   ).
 
 Lemma ctx_init :
-  ctx -∗ seal_pred (N.@"conn".@"init") (session_msg_pred init_pred Init).
+  ctx -∗ seal_pred (N.@"conn".@"init") (session_msg_pred init_pred).
 Proof. solve_ctx. Qed.
 
 Lemma ctx_ack_init :
-  ctx -∗ seal_pred (N.@"conn".@"ack_init") (session_msg_pred ack_init_pred Resp).
+  ctx -∗ seal_pred (N.@"conn".@"ack_init") (session_msg_pred ack_init_pred).
 Proof. solve_ctx. Qed.
 
 Lemma ctx_close :
