store/client_proofs/close.v
@@ -32,9 +32,7 @@ Lemma wp_client_close c kI kR cs :
   store_ctx N -∗
   {{{ db_connected N kI kR cs }}}
     Client.close N c (repr cs)
-  {{{ RET #(); db_disconnected N kI kR ∗
-      (Conn.session_failed cs true ∨ public (si_key cs))
-  }}}.
+  {{{ RET #(); db_disconnected N kI kR ∗ public (si_key cs) }}}.
 Proof.
 iIntros "#chan_c (_ & _ & _ & _ & _ & _ & #?)".
 iIntros "!> %Φ client post".
@@ -42,7 +40,7 @@ iDestruct "client"
   as "(%n & %db & conn & version & #db_at & state & token)".
 wp_lam. wp_pures.
 wp_apply (Conn.wp_close with "[//] [//] [$]").
-iIntros "%failed (#failed & dis & pub)". iApply "post".
+iIntros "(dis & pub)". iApply "post".
 by iFrame.
 Qed.
 
