store/client_proofs/load.v
@@ -7,7 +7,7 @@ From iris.base_logic Require Import invariants.
 From iris.heap_lang Require Import notation proofmode.
 From cryptis Require Import lib term gmeta nown cryptis.
 From cryptis Require Import primitives tactics.
-From cryptis Require Import role conn.
+From cryptis Require Import role iso_dh conn.
 From cryptis.store Require Import impl shared db.
 
 Set Implicit Arguments.
@@ -39,11 +39,13 @@ Lemma wp_client_load c kI kR cs t1 t2 :
       db_connected N kI kR cs ∗
       rem_mapsto N kI kR t1 t2 ∗
       public t2' ∗
-      (Conn.session_failed cs true ∨ ⌜t2' = t2⌝) }}}.
+      (compromised_session Init cs ∨ ⌜t2' = t2⌝) }}}.
 Proof.
 iIntros "#chan_c #ctx #p_t1 !> %Φ [client mapsto] post".
 iDestruct "client"
   as "(%n & %db & conn & version & #db_at & state & token)".
+iAssert (⌜Conn.cs_role cs = Init⌝)%I as "%e_rl".
+{ by iDestruct "token" as "(? & ?)". }
 wp_lam; wp_pures. wp_list.
 iMod (DB.load_client t1 with "version db_at")
   as "(#load_at & version & db)".
@@ -58,9 +60,9 @@ wp_apply (Conn.wp_tick with "conn"). iIntros "conn".
 rewrite [repr_list ts]repr_listE.
 iDestruct "inv_ts" as "[fail|inv_ts]".
 - wp_pures. case: ts => [|t ts]; wp_pures.
-  + iApply "post". iFrame. rewrite public_TInt. by eauto.
+  + iApply "post". iFrame. rewrite public_TInt e_rl. by eauto.
   + rewrite /=. iDestruct "p_ts" as "[p_t _]".
-    iApply "post". iFrame. by eauto.
+    iApply "post". iFrame. rewrite e_rl. by eauto.
 iDestruct "inv_ts" as "(%t1' & %t2' & -> & load_at' & stored_at)".
 iPoseProof (DB.op_at_agree with "load_at load_at'") as "%e".
 case: e => <-.
