store/game.v
@@ -116,14 +116,7 @@ iMod (@client_alloc _ _ _ _ _ _ skR with "tokenI")
   as "(client & free & token)"; eauto.
 wp_apply (wp_client_connect with "[] [] [] [] [] client"); eauto.
 iIntros "%cs client". wp_pure _ credit:"c". wp_pures.
-iPoseProof (db_connected_ok with "client [s_skI s_skR]") as "#>ok".
-{ iIntros "#[fail|fail]".
-  - iPoseProof (sign_key_compromised_keyE with "sign_skI [//]")
-      as ">contra".
-    by iDestruct (secret_not_public with "s_skI contra") as ">[]".
-  - iPoseProof (sign_key_compromised_keyE with "sign_skR [//]")
-      as ">contra".
-    by iDestruct (secret_not_public with "s_skR contra") as ">[]". }
+iPoseProof (db_connected_ok with "client s_skI s_skR [//] [//]") as "#>ok".
 wp_apply wp_recv => //. iIntros "%k #p_k". wp_pures.
 wp_apply wp_recv => //. iIntros "%v #p_v". wp_pures.
 rewrite (@rem_free_at_diff _ _ _ _ _ _ _ {[k]}) //.
@@ -131,28 +124,20 @@ iDestruct "free" as "[free_k free]".
 wp_apply (wp_client_create with "[] [] [] [] [$client $free_k]") => //.
 iIntros "[client k_v]". wp_pures.
 wp_apply (wp_client_close with "[] [] [$client]") => //.
-iIntros "[client [fail|#p_sk]]".
-{ by iPoseProof (Conn.session_failed_agree with "fail ok") as "%". }
+iIntros "[client #p_sk]".
 wp_pures.
 wp_apply Conn.wp_session_key => //. iIntros "_".
 wp_apply (wp_send with "[//]") => //. wp_pures.
 wp_apply (wp_client_connect with "[] [] [] [] [] client"); eauto.
 iIntros "%cs' client". wp_pure _ credit:"c'". wp_pures.
-iPoseProof (db_connected_ok with "client [s_skI s_skR]") as "#>ok'".
-{ iIntros "#[fail|fail]".
-  - iPoseProof (sign_key_compromised_keyE with "sign_skI [//]")
-      as ">contra".
-    by iDestruct (secret_not_public with "s_skI contra") as ">[]".
-  - iPoseProof (sign_key_compromised_keyE with "sign_skR [//]")
-      as ">contra".
-    by iDestruct (secret_not_public with "s_skR contra") as ">[]". }
+iPoseProof (db_connected_ok with "client s_skI s_skR [//] [//]") as "#>#ok'".
 iMod (secret_public with "s_skI") as "#p_skI".
 iMod (secret_public with "s_skR") as "#p_skR".
 wp_apply wp_send => //. wp_pures.
 wp_apply wp_send => //. wp_pures.
 wp_apply (wp_client_load with "[] [] [] [$client $k_v]") => //.
 iIntros "%v' (client & k_v & _ & [fail|->])".
-{ by iPoseProof (Conn.session_failed_agree with "ok' fail") as "%". }
+{ by iPoseProof ("ok'" with "fail") as "[]". }
 wp_pures. wp_apply wp_assert. wp_apply wp_eq_term.
 by rewrite bool_decide_eq_true_2.
 Qed.
